finishing id intro

theories/LogicalRelation/Introductions/Nat.v
@@ -1,5 +1,5 @@
 
-From LogRel Require Import Utils Syntax.All GenericTyping LogicalRelation.
+From LogRel Require Import Utils Syntax.All GenericTyping Monad LogicalRelation.
 From LogRel.LogicalRelation Require Import Properties.
 From LogRel.LogicalRelation.Introductions Require Import Universe SimpleArr Application.
 
@@ -16,8 +16,11 @@ Proof.
   constructor; eapply redtywf_refl; gen_typing.
 Qed.
 
-Definition natRed {Γ l} (wfΓ : [|- Γ]) : [Γ ||-S<l> tNat] :=
+Definition SnatRed {Γ l} (wfΓ : [|- Γ]) : [Γ ||-S<l> tNat] :=
   LRNat_ l (natRedTy wfΓ).
+
+Definition natRed {Γ l} (wfΓ : [|- Γ]) : [Γ ||-<l> tNat] :=
+  WAd_return (SnatRed wfΓ).
 
 
 Lemma natURedTm {Δ} (wfΔ : [|-Δ]) : URedTm zero Δ tNat.
@@ -30,10 +33,10 @@ Lemma natTermRed {Δ} (wfΔ : [|-Δ]) : [Δ ||-<one> tNat : U | LRU_ (redUOneCtx
 Proof.
   unshelve econstructor; try now eapply natURedTm.
   1: cbn; gtyping.
-  eapply redTyRecBwd; now eapply natRed.
+  eapply redTyRecBwd; now eapply SnatRed.
 Defined.
 
-Lemma zeroRed {Γ l A B} {NN : [Γ ||-Nat A ≅ B]} : [Γ ||-<l> tZero : _ | LRNat_ l NN].
+Lemma SzeroRed {Γ l A B} {NN : [Γ ||-Nat A ≅ B]} : [Γ ||-<l> tZero : _ | LRNat_ l NN].
 Proof.
   assert [|-Γ] by (pose (LRNat_ l NN); escape; gtyping).
   exists tZero tZero.
@@ -41,7 +44,13 @@ Proof.
   constructor.
 Defined.
 
-Lemma succRed {Γ l A A' n n'} {NN : [Γ ||-Nat A ≅ A']} :
+Lemma zeroRed {Γ l} (wfΓ : [|-Γ]) : [Γ ||-<l> tZero : _ | natRed (l:=l) wfΓ].
+Proof.
+  unshelve eapply Wpack_return, SirrLR, SzeroRed; tea.
+  2: now eapply natRedTy.
+Qed.
+
+Lemma SsuccRed {Γ l A A' n n'} {NN : [Γ ||-Nat A ≅ A']} :
   [Γ ||-S<l> n ≅ n' : _ | LRNat_ l NN] ->
   [Γ ||-S<l> tSucc n ≅ tSucc n' : _ | LRNat_ l NN].
 Proof.
@@ -52,6 +61,18 @@ Proof.
   + now constructor.
 Defined.
 
+
+Lemma succRed {Γ l n n'} (wfΓ : [|-Γ]) :
+  [Γ ||-<l> n ≅ n' : _ | natRed (l:=l) wfΓ] ->
+  [Γ ||-<l> tSucc n ≅ tSucc n' : _ | natRed (l:=l) wfΓ].
+Proof.
+  intros Rn.
+  eapply (Split_bind_return Rn).
+  intros Δ wfΔ ρ oRn oirr; cbn.
+  unshelve (now eapply SirrLR, SsuccRed, SirrLR, Rn).
+  3: eapply natRedTy.
+  all: tea.
+Qed.
 
 Lemma elimSuccHypTy_subst {P} σ :
   elimSuccHypTy P[up_term_term σ] = (elimSuccHypTy P)[σ].
@@ -67,7 +88,7 @@ Qed.
 Lemma liftSubst_singleSubst_eq {t u v: term} : t[u]⇑[v..] = t[u[v..]..].
 Proof. now bsimpl. Qed.
 
-Section NatElimRedEq.
+Section SNatElimRedEq.
   Context {Γ l P Q hs hs' hz hz'}
     (NN : [Γ ||-Nat tNat ≅ tNat])
     (RN := LRNat_ _ NN)
@@ -75,36 +96,36 @@ Section NatElimRedEq.
     (WtQ : [Γ ,, tNat |- Q])
     (eqPQ : [Γ,, tNat |- P ≅ Q])
     (RPQext : forall n n' (Rn : [Γ ||-S<l> n ≅ n' : _ | RN]),
-      [Γ ||-S<l> P[n..] ≅ Q[n'..]])
-    (RPQz := RPQext _ _ zeroRed)
-    (Rhz : [Γ ||-S<l> hz ≅ hz' : _ | RPQz])
-    (RPQs : [Γ ||-S<l> elimSuccHypTy P ≅ elimSuccHypTy Q])
-    (Rhs : [Γ ||-S<l> hs ≅ hs' : _ | RPQs ]) .
+      [Γ ||-<l> P[n..] ≅ Q[n'..]])
+    (RPQz := RPQext _ _ SzeroRed)
+    (Rhz : [Γ ||-<l> hz ≅ hz' : _ | RPQz])
+    (RPQs : [Γ ||-<l> elimSuccHypTy P ≅ elimSuccHypTy Q])
+    (Rhs : [Γ ||-<l> hs ≅ hs' : _ | RPQs ]) .
 
-  #[local]
-  Lemma RPext : forall n n' (Rn : [Γ ||-S<l> n ≅ n' : _ | RN]),
-      [Γ ||-S<l> P[n..] ≅ P[n'..]].
+  Let RPext : forall n n' (Rn : [Γ ||-S<l> n ≅ n' : _ | RN]),
+      [Γ ||-<l> P[n..] ≅ P[n'..]].
   Proof.
     intros; etransitivity; [|symmetry];  eapply RPQext; tea; now eapply urefl.
   Qed.
 
-  Lemma natElimRedEqAux :
+  Lemma SnatElimRedEqAux :
     (forall n n' (Rnn' : [Γ ||-S<l> n ≅ n' : _ | RN]),
-      [Γ ||-<l> tNatElim P hz hs n ≅ tNatElim Q hz' hs' n' : _ | WAd_return (RPQext _ _ Rnn') ]) ×
-    (forall n n' (Rnn' : NatPropEq Γ n n') (RP : [Γ ||-S<l> P[n..] ≅ Q[n'..]]),
-      [Γ ||-<l> tNatElim P hz hs n ≅ tNatElim Q hz' hs' n' : _ | WAd_return RP ]).
-  Proof. 
+      [Γ ||-<l> tNatElim P hz hs n ≅ tNatElim Q hz' hs' n' : _ | RPQext _ _ Rnn' ]) ×
+    (forall n n' (Rnn' : NatPropEq Γ n n') (RP : [Γ ||-<l> P[n..] ≅ Q[n'..]]),
+      [Γ ||-<l> tNatElim P hz hs n ≅ tNatElim Q hz' hs' n' : _ | RP ]).
+  Proof.
+    eassert ([|-Γ]) as wfΓ by (escape; gtyping).
     apply NatRedEqInduction.
     - intros t u  nfL nfR redL redR ? prop ih.
       set (Rtu := Build_NatRedTmEq _ _ _ _ _ _ : [Γ ||-S<l> t ≅ u : _ | RN]).
       pose proof (redTmFwd' Rtu) as []; eapply redSubstTmEq.
       + unshelve eapply irrLRConv, ih;
-        first [eapply RPQext| eapply WAd_return, RPext]; tea; now symmetry.
+        first [eapply RPQext| eapply RPext]; tea; now symmetry.
       + escape; eapply redtm_natelim; tea; gen_typing.
       + escape; eapply redtm_natelim; tea; [..| gtyping].
         1,2: now eapply ty_conv.
     - intros; eapply redSubstTmEq.
-      + eapply Wpack_return,SirrLR, Rhz.
+      + eapply irrLR, Rhz.
       + escape; eapply redtm_natElimZero; tea.
       + escape; eapply redtm_natElimZero; tea.
         1,2: now eapply ty_conv.
@@ -114,26 +135,93 @@ Section NatElimRedEq.
       + escape; eapply redtm_natElimSucc; tea.
         1,2: now eapply ty_conv.
       + assert [Γ ||-<l> arr P[n..] P[(tSucc n)..] ≅ arr Q[n'..] Q[(tSucc n')..]].
-        1: now eapply WAd_return, ArrRedTy; eapply RPQext;[|eapply succRed].
-        unshelve eapply simple_appcongTerm'; [..| eauto]; tea.
-        unshelve (eapply irrLREq, appcongTerm; tea; now rewrite subst_arr, liftSubst_singleSubst_eq); tea.
+        1: now eapply ArrRedTy; eapply RPQext;[|eapply SsuccRed].
+        unshelve eapply simple_appcongTerm; [..| eauto]; tea.
+        eapply Wpack_return in Rn as WRn.
+        unshelve (eapply irrLREq, appcongTerm; tea;
+          now rewrite subst_arr, liftSubst_singleSubst_eq); tea.
         now rewrite 2!subst_arr, 2!liftSubst_singleSubst_eq.
     - intros n n' Rn RP0.
-      pose proof (neNfTermEq RN Rn).
-      eapply Wpack_return, reflectLR.
-      + escape; now eapply ty_natElim.
-      + eapply ty_conv ; [| eapply escapeEq; now symmetry].
-        escape; eapply ty_natElim; tea.
-        all: now eapply ty_conv.
-      + escape ; destruct Rn; now eapply convneu_natElim.
+      epose proof (SneNfTermEq RN Rn).
+      escape.
+      eapply irrLR.
+      eapply neNfTermEq; constructor.
+      + now eapply ty_natElim.
+      + eapply ty_conv.
+        eapply ty_natElim; tea.
+        * now eapply ty_conv.
+        * now eapply ty_conv.
+        * now symmetry.
+      + destruct Rn; now eapply convneu_natElim.
+      Unshelve.
+      2: now eapply lrefl.
   Qed.
 
-  Lemma natElimRedEq :
+  Lemma SnatElimRedEq :
     (forall n n' (Rnn' : [Γ ||-S<l> n ≅ n' : _ | RN]),
-      [Γ ||-<l> tNatElim P hz hs n ≅ tNatElim Q hz' hs' n' : _ | WAd_return  (RPQext _ _ Rnn') ]).
-  Proof. intros; now apply (fst natElimRedEqAux). Qed.
+      [Γ ||-<l> tNatElim P hz hs n ≅ tNatElim Q hz' hs' n' : _ |  (RPQext _ _ Rnn') ]).
+  Proof. intros; now apply (fst SnatElimRedEqAux). Qed.
+End SNatElimRedEq.
+
+Section NatElimRedEq.
+  Context {Γ l P Q}
+    (wfΓ : [|- Γ])
+    (WtP : [Γ ,, tNat |- P])
+    (WtQ : [Γ ,, tNat |- Q])
+    (eqPQ : [Γ,, tNat |- P ≅ Q])
+    (RPQext : forall Δ (wfΔ : [|-Δ]) (ρ : Δ ≤ Γ) n n' (Rn : [Δ ||-<l> n ≅ n' : _ | natRed (l:=l) wfΔ ]),
+      [Δ ||-<l> P⟨wk_up tNat ρ⟩[n..] ≅ Q⟨wk_up tNat ρ⟩[n'..]]).
+
+
+  Let RPQextnow : forall n n',
+    [Γ ||-<l> n ≅ n' : _ | natRed (Γ := Γ) (l:=l) wfΓ] -> [Γ ||-<l> P[n..] ≅ Q[n'..]].
+  Proof.
+    intros n n' Rnn'.
+    epose (RPQ := RPQext Γ wfΓ wk_id n n' Rnn').
+    replace P with P⟨wk_id (Γ:=Γ,,tNat)⟩ by eapply wk_id_ren_on.
+    now replace Q with Q⟨wk_id (Γ:=Γ,,tNat)⟩ by eapply wk_id_ren_on.
+  Qed.
+
+  Context {hs hs' hz hz'}
+    (RPQz := RPQextnow _ _ (zeroRed wfΓ))
+    (Rhz : [Γ ||-<l> hz ≅ hz' : _ | RPQz])
+    (RPQs : [Γ ||-<l> elimSuccHypTy P ≅ elimSuccHypTy Q])
+    (Rhs : [Γ ||-<l> hs ≅ hs' : _ | RPQs ]).
+
+  Let RPext : forall Δ (wfΔ : [|-Δ]) (ρ : Δ ≤ Γ) n n' (Rn : [Δ ||-<l> n ≅ n' : _ | natRed (l:=l) wfΔ]),
+      [Δ ||-<l> P⟨wk_up tNat ρ⟩[n..] ≅ P⟨wk_up tNat ρ⟩[n'..]].
+  Proof.
+    intros; etransitivity; [|symmetry];  eapply RPQext; tea; now eapply urefl.
+  Qed.
+
+
+  Lemma natElimRedEq n n' (Rnn' : [Γ ||-<l> n ≅ n' : _ | natRed wfΓ]):
+      [Γ ||-<l> tNatElim P hz hs n ≅ tNatElim Q hz' hs' n' : _ | RPQextnow _ _ Rnn' ].
+  Proof.
+    eapply (dSplit_bind Rnn').
+    intros Δ wfΔ ρ oRN oRnn'.
+    eapply Wpackrefold.
+    eassert [|-Δ,,tNat] as wfΔN by (eapply wfc_cons; gtyping).
+    rewrite <- 2wk_natElim.
+    eapply irrLREq, SnatElimRedEq; refold.
+    1: symmetry; eapply subst_ren_wk_up.
+    Unshelve.
+    + now eapply wft_wk.
+    + now eapply wft_wk.
+    + now eapply convty_wk.
+    + unshelve eapply irrLREq, wkLRTm, Rhz; tea.
+      exact (subst_ren_wk_up _).
+    + unshelve eapply irrLREq, wkLRTm, Rhs; tea.
+      symmetry; eapply wk_elimSuccHypTy.
+    + easy.
+    + now eapply natRedTy.
+    + clear dependent n; clear n'; intros n n' Rnn'.
+      eapply (RPQext _ wfΔ), Wpack_return, SirrLR, Rnn'.
+    + now unshelve now eapply SirrLREq, Rnn'.
+    + rewrite 2 wk_elimSuccHypTy.
+      now eapply wkLRTy.
+  Qed.
+
 End NatElimRedEq.
-
-
 
 End Nat.
