theories/LogicalRelation/Introductions/Empty.v
@@ -1,4 +1,4 @@
-From LogRel Require Import Utils Syntax.All GenericTyping LogicalRelation.
+From LogRel Require Import Utils Syntax.All GenericTyping Monad LogicalRelation.
 From LogRel.LogicalRelation Require Import Properties.
 From LogRel.LogicalRelation.Introductions Require Import Universe SimpleArr Application.
 From Equations Require Import Equations.
@@ -13,8 +13,11 @@ Context `{GenericTypingProperties}.
 Lemma emptyRedTy {Γ} : [|- Γ] -> [Γ ||-Empty tEmpty ≅ tEmpty].
 Proof. intros; constructor; eapply redtywf_refl; gen_typing. Defined.
 
-Lemma emptyRed {Γ l} : [|- Γ] -> [Γ ||-S<l> tEmpty].
+Lemma SemptyRed {Γ l} : [|- Γ] -> [Γ ||-S<l> tEmpty].
 Proof. intros; now apply LREmpty_, emptyRedTy. Defined.
+
+Lemma emptyRed {Γ l} : [|- Γ] -> [Γ ||-<l> tEmpty].
+Proof. intros wfΓ. now eapply WAd_return, SemptyRed. Defined.
 
 Lemma emptyURedTm {Δ l} (wfΔ : [|-Δ]) : URedTm l Δ tEmpty.
 Proof.
@@ -26,43 +29,98 @@ Lemma emptyTermRed {Δ} (wfΔ : [|-Δ]) : [Δ ||-<one> tEmpty : U | LRU_ (redUOn
 Proof.
   unshelve eexists (emptyURedTm wfΔ) (emptyURedTm wfΔ); cbn.
   1: gtyping.
-  now eapply (emptyRed (l:=zero)).
+  now eapply (SemptyRed (l:=zero)).
 Defined.
 
-Section EmptyElimRedEq.
+
+
+
+Section SEmptyElimRedEq.
   Context {Γ l P Q}
     (wfΓ : [|- Γ])
     (NN : [Γ ||-Empty tEmpty ≅ tEmpty])
-    (RN := LREmpty_ _ NN)
+    (RN := LREmpty_ l NN)
     (WtP : [Γ,, tEmpty |- P])
     (WtQ : [Γ,, tEmpty |- Q])
     (eqPQ : [Γ,, tEmpty |- P ≅ Q])
-    (RPQext : forall n n', [Γ ||-S<l> n ≅ n' : _ | RN] -> [Γ ||-S<l> P[n..] ≅ Q[n'..]]).
+    (RPQext : forall n n', [Γ ||-S<l> n ≅ n' : _ | RN] -> [Γ ||-<l> P[n..] ≅ Q[n'..]]).
 
-  #[local]
-  Lemma RPext : forall n n' (Rn : [Γ ||-<l> n ≅ n' : _ | RN]),
-      [Γ ||-S<l> P[n..] ≅ P[n'..] ].
+  Let RPext : forall n n' (Rn : [Γ ||-S<l> n ≅ n' : _ | RN]),
+      [Γ ||-<l> P[n..] ≅ P[n'..] ].
   Proof.
     intros; etransitivity; [|symmetry];  eapply RPQext; tea; now eapply urefl.
   Qed.
 
-  Lemma emptyElimRedEq n n' (Rnn' : [Γ ||-<l> n ≅ n' : _ | RN]) :
-    [Γ ||-<l> tEmptyElim P n ≅ tEmptyElim Q n' : _ | RPQext _ _ Rnn' ].
+
+  Lemma SemptyElimRedEq n n' (Rnn' : [Γ ||-S<l> n ≅ n' : _ | RN])
+    (RPQ : [Γ ||-<l> P[n..] ≅ Q[n'..]]):
+    [Γ ||-<l> tEmptyElim P n ≅ tEmptyElim Q n' : _ | RPQ ].
   Proof.
     pose proof (redTmFwd' Rnn') as [].
-    depelim Rnn' ; eapply SredSubstTmEq; cycle 1.
+    depelim Rnn' ; eapply redSubstTmEq; cycle 1.
     + eapply redtm_emptyelim; tea; gen_typing.
     + eapply redtm_emptyelim; tea; gen_typing.
-    + destruct eq; eapply SirrLRConv.
+    + cbn -[Wpack] in e,e0,e1.
+     destruct eq; eapply irrLRConv.
       (* gtyping/gen_typing not working well here... *)
       2: eapply neNfTermEq; constructor; [now eapply ty_emptyElim |..].
       - eapply RPext; now symmetry.
       - eapply ty_conv; [now eapply ty_emptyElim|].
-        symmetry; now eapply escapeEq, RPQext.
+        symmetry; now eapply escapeSplitTy, RPQext.
       - now eapply convneu_emptyElim.
       Unshelve. now eapply lrefl, RPQext.
   Qed.
+End SEmptyElimRedEq.
+
+
+
+Section EmptyElimRedEq.
+  Context {Γ l P Q}
+    (wfΓ : [|- Γ])
+    (WtP : [Γ,, tEmpty |- P])
+    (WtQ : [Γ,, tEmpty |- Q])
+    (eqPQ : [Γ,, tEmpty |- P ≅ Q])
+    (RPQext : forall Δ wfΔ (ρ : Δ ≤Γ) n n',
+      [Δ ||-<l> n ≅ n' : _ | emptyRed (Γ := Δ) (l:=l) wfΔ] -> [Δ ||-<l> P⟨wk_up tEmpty ρ⟩[n..] ≅ Q⟨wk_up tEmpty ρ⟩[n'..]]).
+
+  Let RPext : forall Δ wfΔ (ρ : Δ ≤Γ) n n' (Rn : [Δ ||-<l> n ≅ n' : _ | emptyRed (Γ := Δ) (l:=l) wfΔ]),
+      [Δ ||-<l> P⟨wk_up tEmpty ρ⟩[n..] ≅ P⟨wk_up tEmpty ρ⟩[n'..] ].
+  Proof.
+    intros; etransitivity; [|symmetry];  eapply RPQext; tea; now eapply urefl.
+  Qed.
+
+  Let RPQextnow : forall n n', [Γ ||-<l> n ≅ n' : _ | emptyRed (Γ := Γ) (l:=l) wfΓ] -> [Γ ||-<l> P[n..] ≅ Q[n'..]].
+  Proof.
+    intros n n' Rnn'.
+    epose (RPQ := RPQext Γ wfΓ wk_id n n' Rnn').
+    replace P with P⟨wk_id (Γ:=Γ,,tEmpty)⟩ by eapply wk_id_ren_on.
+    now replace Q with Q⟨wk_id (Γ:=Γ,,tEmpty)⟩ by eapply wk_id_ren_on.
+  Qed.
+
+
+  Lemma emptyElimRedEq n n' (Rnn' : [Γ ||-<l> n ≅ n' : _ | emptyRed wfΓ]) :
+    [Γ ||-<l> tEmptyElim P n ≅ tEmptyElim Q n' : _ | RPQextnow _ _ Rnn' ].
+  Proof.
+    eapply (dSplit_bind Rnn').
+    intros Δ wfΔ ρ oRN oRnn'.
+    eapply Wpackrefold.
+    eassert [|-Δ,,tEmpty] as wfΔE by (eapply wfc_cons; gtyping).
+    rewrite <- 2wk_emptyElim.
+    eapply irrLREq, SemptyElimRedEq; refold.
+    1: symmetry; eapply subst_ren_wk_up.
+    Unshelve.
+    + now eapply wft_wk.
+    + now eapply wft_wk.
+    + now eapply convty_wk.
+    + clear dependent n; clear n'; intros n n' Rnn'.
+      eapply (RPQext _ wfΔ), Wpack_return, SirrLR, Rnn'.
+    + now unshelve now eapply SirrLREq, Rnn'.
+    + easy.
+    + now unshelve now eapply RPQext, irrLREq, wkLRTm, Rnn'.
+    + now eapply emptyRedTy.
+  Qed.
 End EmptyElimRedEq.
+
 
 End Empty.
 
