theories/LogicalRelation/Introductions/Id.v
@@ -1,4 +1,4 @@
-From LogRel Require Import Utils Syntax.All GenericTyping LogicalRelation.
+From LogRel Require Import Utils Syntax.All GenericTyping Monad LogicalRelation.
 From LogRel.LogicalRelation Require Import Properties.
 From LogRel.LogicalRelation.Introductions Require Import Universe.
 
@@ -19,14 +19,31 @@ Section IdRed.
     typeclasses eauto.
   Defined.
 
-  Lemma IdRed {Γ l A A' t t' u u'} (RA : [Γ ||-S<l> A ≅ A']) :
+  Lemma SIdRed {Γ l A A' t t' u u'} (RA : [Γ ||-S<l> A ≅ A']) :
       [RA | Γ ||- t ≅ t' : _] ->
       [RA | Γ ||- u ≅ u' : _] ->
       [Γ ||-S<l> tId A t u ≅ tId A' t' u'].
   Proof. intros; apply LRId'; now eapply IdRed0. Defined.
 
+  Lemma IdRed {Γ l A A' t t' u u'} (RA : [Γ ||-<l> A ≅ A']) :
+      [RA | Γ ||- t ≅ t' : _] ->
+      [RA | Γ ||- u ≅ u' : _] ->
+      [Γ ||-<l> tId A t u ≅ tId A' t' u'].
+  Proof.
+    intros Rt Ru.
+    eapply (Split_bind Rt).
+    intros Δ wfΔ ρ oRt.
+    eapply (dSplit_wk_bind_return Ru wfΔ ρ).
+    intros Ξ wfΞ ρΞ oRA oRu.
+    rewrite <- 2wk_Id.
+    unshelve eapply SIdRed.
+    + now eapply RA.
+    + now eapply Rt, overtree_PSh.
+    + now eapply Ru.
+  Qed.
 
-  Lemma IdCongRedU@{i j k l} {Γ l A A' t t' u u'}
+
+  Lemma SIdCongRedU@{i j k l} {Γ l A A' t t' u u'}
       (RU : [LogRel@{i j k l} l | Γ ||- U ≅ U])
       (RU' := invLRU RU)
       (RA : [LogRel@{i j k l} (URedTy.level RU') | Γ ||- A ≅ A']) :
@@ -42,13 +59,38 @@ Section IdRed.
     2,4: constructor.
     1,2: eapply redtmwf_refl.
     1-3: gtyping.
-    unshelve eapply redTyRecBwd, IdRed.
+    unshelve eapply redTyRecBwd, SIdRed.
     1: now eapply cumLR.
     all: now eapply SirrLR.
   Qed.
 
 
-Lemma reflCongRed0 {Γ l A A0 A' B x x'}
+  Lemma IdCongRedU@{i j k l} {Γ l l' A A' t t' u u'}
+      (RU : WLRAdequate@{i j k l} Γ l U U)
+      (RA : [RU | _ ||- A ≅ A' : U])
+      (RA' := UnivEq l' RU RA) :
+    [RA' | _ ||- t ≅ t' : _] ->
+    [RA' | _ ||- u ≅ u' : _] ->
+    [RU | _ ||- tId A t u ≅ tId A' t' u' : U].
+  Proof.
+    intros Rt Ru.
+    eapply (Split_bind RA).
+    intros Δ wfΔ ρ oRA.
+    eapply (Split_wk_bind Rt wfΔ ρ).
+    intros Ξ wfΞ ρΞ oRt.
+    eapply (dSplit_wk_bind_return Ru wfΞ (ρΞ ∘w ρ)).
+    intros Θ wfΘ ρΘ oRA' oRu oRU.
+    cbn -[wk_well_wk_compose].
+    unshelve eapply SIdCongRedU.
+    + now unshelve now eapply SUnivEq, RA, overtree_PSh, overtree_PSh.
+    + now unshelve now eapply RA, overtree_PSh, overtree_PSh.
+    + unshelve eapply SirrLRCum, Rt, overtree_PSh, oRt; tea.
+      now eapply lrefl, RA'.
+    + unshelve eapply SirrLRCum, Ru, oRu; tea.
+      now eapply lrefl, RA'.
+Qed.
+
+Lemma SreflCongRed0 {Γ l A A0 A' B x x'}
   (RA : [Γ ||-S<l> A ≅ A0])
   (wfA' : [Γ |- A'])
   (eqA : [Γ |- A ≅ A'])
@@ -71,10 +113,36 @@ Proof.
   all: first [now eapply SirrLREq| now eapply lrefl, SirrLREq].
 Qed.
 
-Lemma reflCongRed {Γ l A A' x x'}
+Lemma reflCongRed0 {Γ l A A0 A' B x x'}
+  (RA : [Γ ||-<l> A ≅ A0])
+  (wfA' : [Γ |- A'])
+  (eqA : [Γ |- A ≅ A'])
+  (Rxx : [RA | _ ||- x ≅ x' : _])
+  (RIA : [Γ ||-<l> tId A x x ≅ B]) :
+  [RIA | _ ||- tRefl A x ≅ tRefl A' x' : _].
+Proof.
+  eapply (dSplit_bind_return Rxx).
+  intros * oRA oRxx oRIA.
+  cbn.
+  eapply SreflCongRed0; refold.
+  + now eapply wft_wk.
+  + now eapply convty_wk.
+  + now unshelve now eapply Rxx.
+Qed.
+
+Lemma SreflCongRed {Γ l A A' x x'}
   (RA : [Γ ||-S<l> A ≅ A'])
   (Rxx : [RA | _ ||- x ≅ x' : _])
   (RIA : [Γ ||-S<l> tId A x x ≅ tId A' x' x']) :
+  [RIA | _ ||- tRefl A x ≅ tRefl A' x' : _].
+Proof.
+  escape; now eapply SreflCongRed0.
+Qed.
+
+Lemma reflCongRed {Γ l A A' x x'}
+  (RA : [Γ ||-<l> A ≅ A'])
+  (Rxx : [RA | _ ||- x ≅ x' : _])
+  (RIA : [Γ ||-<l> tId A x x ≅ tId A' x' x']) :
   [RIA | _ ||- tRefl A x ≅ tRefl A' x' : _].
 Proof.
   escape; now eapply reflCongRed0.
@@ -91,7 +159,7 @@ Lemma reflCongRed' {Γ l A Al Ar x xl xr}
   (Rxxr : [RA | _ ||- x ≅ xr : _])
   (RIA : [Γ ||-S<l> tId A x x]) :
   [RIA | _ ||- tRefl Al xl ≅ tRefl Ar xr : _].
-Proof. etransitivity; [symmetry|]; now eapply (reflCongRed0 RA), SirrLR. Qed.
+Proof. etransitivity; [symmetry|]; now eapply (SreflCongRed0 RA), SirrLR. Qed.
 
 Lemma idElimPropCongRed {Γ l A A' x x' P P' hr hr' y y' e e'}
   (RA : [Γ ||-S<l> A ≅ A'])
@@ -104,8 +172,8 @@ Lemma idElimPropCongRed {Γ l A A' x x' P P' hr hr' y y' e e'}
     (Ryy' : [RA | _ ||- y ≅ y' : _])
     {RIAxy : [Γ ||-S<l> tId A x y ≅ tId A' x' y']}
     (Ree' : [ RIAxy | _ ||- e ≅ e' : _]),
-    [Γ ||-S<l> P[e .: y..] ≅ P'[e' .: y'..]])
-  (Rrfl := (reflCongRed RA Rxx' RIAxx))
+    [Γ ||-<l> P[e .: y..] ≅ P'[e' .: y'..]])
+  (Rrfl := (SreflCongRed RA Rxx' RIAxx))
   (Rhrhr' : [RP Rxx' Rrfl | _ ||- hr ≅ hr' : _])
   (Ryy' : [RA | _ ||- y ≅ y' : _])
   (RIAxy : [Γ ||-S<l> tId A x y ≅ tId A' x' y'])
@@ -115,8 +183,8 @@ Lemma idElimPropCongRed {Γ l A A' x x' P P' hr hr' y y' e e'}
 Proof.
   pose proof (RP _ _ _ _ Rxx' _ Rrfl).
   pose proof (RP _ _ _ _ Ryy' _ Ree').
-  destruct Pee' as [B B' z z' ?????? xz xz' yz yz'|]; cbn in *; escape.
-  - eapply SredSubstTmEq; cycle 1.
+  destruct Pee' as [B B' z z' ?????? xz xz' yz yz'|]; cbn -[Wpack] in *; escape.
+  - eapply redSubstTmEq; cycle 1.
     + eapply redtm_idElimRefl; tea.
       transitivity z; [|symmetry]; tea.
     + eapply redtm_idElimRefl; tea.
@@ -128,21 +196,25 @@ Proof.
       transitivity x; tea; now symmetry.
     + assert [RA | _ ||- x ≅ y' : _].
       1: transitivity y; tea; transitivity z; [|symmetry]; now eapply SirrLR.
-      eapply SirrLRConv; tea.
+      eapply irrLRConv; tea.
       unshelve (etransitivity; [|symmetry]; eapply RP; cycle 3; tea).
-      1: now eapply IdRed.
-      now eapply reflCongRed0.
-  - eapply reflectLR.
+      1: now eapply SIdRed.
+      now eapply SreflCongRed0.
+  - (* pose proof (SneNfTermEq RN r). *)
+    eapply irrLR.
+    eapply neNfTermEq; constructor.
     + now eapply ty_IdElim.
     + eapply ty_conv; [|symmetry; tea].
       eapply ty_IdElim; tea.
       all: eapply ty_conv; tea.
     + eapply convneu_IdElim; tea.
       destruct r;  now cbn in *.
+    Unshelve.
+    2: now eapply lrefl.
 Qed.
 
 
-Lemma idElimCongRed {Γ l A A' x x' P P' hr hr' y y' e e'}
+Lemma SidElimCongRed {Γ l A A' x x' P P' hr hr' y y' e e'}
   (RA : [Γ ||-S<l> A ≅ A'])
   (Rxx' : [RA | _ ||- x ≅ x' : _])
   (RIAxx : [Γ ||-S<l> tId A x x ≅ tId A' x' x'])
@@ -153,8 +225,8 @@ Lemma idElimCongRed {Γ l A A' x x' P P' hr hr' y y' e e'}
     (Ryy' : [RA | _ ||- y ≅ y' : _])
     {RIAxy : [Γ ||-S<l> tId A x y ≅ tId A' x' y']}
     (Ree' : [ RIAxy | _ ||- e ≅ e' : _]),
-    [Γ ||-S<l> P[e .: y..] ≅ P'[e' .: y'..]])
-  (Rrfl := (reflCongRed RA Rxx' RIAxx))
+    [Γ ||-<l> P[e .: y..] ≅ P'[e' .: y'..]])
+  (Rrfl := (SreflCongRed RA Rxx' RIAxx))
   (Rhrhr' : [RP Rxx' Rrfl | _ ||- hr ≅ hr' : _])
   (Ryy' : [RA | _ ||- y ≅ y' : _])
   (RIAxy : [Γ ||-S<l> tId A x y ≅ tId A' x' y'])
@@ -163,8 +235,8 @@ Lemma idElimCongRed {Γ l A A' x x' P P' hr hr' y y' e e'}
 Proof.
   assert (nRee' : [LRId' (normRedId RIAxy) | Γ ||- e ≅ e' : _]) by now eapply SirrLREq.
   pose proof (redTmFwd' nRee') as [].
-  eapply SredSubstTmEq.
-  + eapply SirrLRConv.
+  eapply redSubstTmEq.
+  + eapply irrLRConv.
     2: unshelve (eapply idElimPropCongRed; cycle 4; [exact (nRee'.(IdRedTmEq.prop))| tea..]); tea.
     2: now eapply SirrLR.
     etransitivity; [|symmetry]; eapply RP; cycle 1; [now eapply lrefl| tea..].
@@ -173,9 +245,40 @@ Proof.
     1,3: now eapply ty_conv.
     2: eapply redtm_conv; [eapply tmr_wf_red; exact (whredtmR nRee').(tmred_whnf_red)|].
     2: unfold IdRedTy.outTy; cbn; gtyping.
-    eapply ty_conv; tea; eapply escapeEq, RP; tea.
+    eapply ty_conv; tea; eapply escapeSplitTy , RP; tea.
 Qed.
 
 
+Lemma idElimCongRed {Γ l A A' x x' P P' hr hr' y y' e e'}
+  (RA : [Γ ||-<l> A ≅ A'])
+  (Rxx' : [RA | _ ||- x ≅ x' : _])
+  (RIAxx := IdRed RA Rxx' Rxx')
+  (RP0 : [Γ ,, A ,, tId A⟨@wk1 Γ A⟩ x⟨@wk1 Γ A⟩ (tRel 0) |- P])
+  (RP0' : [Γ ,, A' ,, tId A'⟨@wk1 Γ A'⟩ x'⟨@wk1 Γ A'⟩ (tRel 0) |- P'])
+  (RPP0 : [Γ ,, A ,, tId A⟨@wk1 Γ A⟩ x⟨@wk1 Γ A⟩ (tRel 0) |- P ≅ P'])
+  (RP : forall {y y' e e'}
+    (Ryy' : [RA | _ ||- y ≅ y' : _])
+    (Ree' : [ IdRed RA Rxx' Ryy'| _ ||- e ≅ e' : _]),
+    [Γ ||-<l> P[e .: y..] ≅ P'[e' .: y'..]])
+  (Rrfl := (reflCongRed RA Rxx' RIAxx))
+  (Rhrhr' : [RP Rxx' Rrfl | _ ||- hr ≅ hr' : _])
+  (Ryy' : [RA | _ ||- y ≅ y' : _])
+(*   (RIAxy : [Γ ||-<l> tId A x y ≅ tId A' x' y']) *)
+  (Ree' : [IdRed RA Rxx' Ryy' | _ ||- e ≅ e' : _]) :
+  [RP Ryy' Ree' | _ ||- tIdElim A x P hr y e ≅ tIdElim A' x' P' hr' y' e' : _].
+Proof.
+  eapply (Split_bind Rxx').
+  intros Δ wfΔ ρ oRxx'.
+  eapply (Wpackrefold wfΔ), (dSplit_wk_bind Ryy' wfΔ ρ).
+  intros Ξ wfΞ ρΞ oRA oRyy'.
+  eapply (Wpackrefold wfΞ), (dSplit_wk_bind Ree' wfΞ (ρΞ∘w ρ)).
+  intros Θ wfΘ ρΘ oIdRed oRee'; eapply (Wpackrefold wfΘ).
+  rewrite 2(wk_comp_ren_on (tIdElim A' x' P' hr' y' e')),
+    2(wk_comp_ren_on (tIdElim A x P hr y e)).
+  rewrite <- wk_idElim.
+  eapply irrLREq, SidElimCongRed;refold.
+  1: now rewrite 2 (wk_comp_ren_on P[e .: y..]), <- subst_ren_wk_up2.
+  +
+    
 
 End IdRed.
